theories/Languages/Semantics.v
@@ -1,6 +1,8 @@
 Set Default Goal Selector "!".
 
+From Stdlib Require Import ZArith.
 From Stdlib Require Import Nat.
+From Reactive.Datatypes Require Dict Stream.
 From Reactive.Props Require Import Identifier Sigma.
 
 Inductive type : Set :=
@@ -111,165 +113,201 @@ Proof.
 Qed.
 
 Inductive const : type -> Set :=
-  | CVoid: const TVoid
   | CBool: bool -> const TBool
-  | CInt: nat -> const TInt
+  | CInt: Z -> const TInt
 .
 Lemma const_inv {ty} (x: const ty) :
   {eq : ty = _ & {b : bool | x = eq_rect _ const (CBool b) _ (eq_sym eq)}} +
-  {eq : ty = _ & {n : nat | x = eq_rect _ const (CInt n) _ (eq_sym eq)}} +
-  {exists (eq : ty = _), x = eq_rect _ const CVoid _ (eq_sym eq)}.
+  {eq : ty = _ & {n : Z | x = eq_rect _ const (CInt n) _ (eq_sym eq)}}.
 Proof using.
-  destruct x as [|b|n]; [right|left; left|left; right]; exists eq_refl; [|exists b|exists n]; exact eq_refl.
+  destruct x as [b|n]; [left|right]; exists eq_refl; [exists b|exists n]; exact eq_refl.
 Defined.
 
 Lemma const_dec {ty} (x y: const ty) : {x = y} + {x <> y}.
 Proof.
-  destruct x as [ | b | n ].
-  all: destruct (const_inv y) as [[[eq' [b' ->]]|[eq' [n' ->]]]|H].
+  destruct x as [b | n ].
+  all: destruct (const_inv y) as [[eq' [b' ->]]|[eq' [n' ->]]].
   all: try discriminate; try solve [right; destruct H as [f _]; discriminate f].
-  1: left; destruct H as [eq' ->].
-  2: destruct (Bool.bool_dec b b') as [eq|ne]; [left|right].
-  4: destruct (PeanoNat.Nat.eq_dec n n') as [eq|ne]; [left|right].
+  1: destruct (Bool.bool_dec b b') as [eq|ne]; [left|right].
+  3: destruct (Z.eq_dec n n') as [eq|ne]; [left|right].
   all: rewrite !(Eqdep_dec.UIP_dec type_dec _ eq_refl); cbn; try intros [=f]; auto.
-  exact (f_equal _ eq).
+  all: exact (f_equal _ eq).
 Defined.
 
+Definition const_eqb {ty1} (c1: const ty1) {ty2} (c2: const ty2): bool :=
+  match c1, c2 with
+    | CBool b1, CBool b2 => Bool.eqb b1 b2
+    | CInt n1, CInt n2 => Z.eqb n1 n2
+    | _, _ => false
+  end.
+
+Lemma const_eqb_refl {ty} (c: const ty):
+  const_eqb c c = true.
+Proof.
+  destruct c as [ b | n ].
+  - apply Bool.eqb_true_iff.
+    reflexivity.
+  - apply Z.eqb_refl.
+Qed.
+
 Inductive value : type -> Set :=
-  | VConst : forall {ty}, const ty -> value ty
-  | VIfte  : forall {ty}, value TBool -> value ty -> value ty -> value ty
-  | Vnot   : value TInt -> value TInt
-  | Vneg   : value TInt -> value TInt
-  | Vand   : value TBool -> value TBool -> value TBool
-  | Vor    : value TBool -> value TBool -> value TBool
-  | Vxor   : value TBool -> value TBool -> value TBool
-  | Vplus  : value TInt -> value TInt -> value TInt
-  | Vminus : value TInt -> value TInt -> value TInt
-  | Vmult  : value TInt -> value TInt -> value TInt
-  | Vdiv   : value TInt -> value TInt -> value TInt
-  | Veq    : value TInt -> value TInt -> value TBool
-  | Vneq   : value TInt -> value TInt -> value TBool
-  | Vle    : value TInt -> value TInt -> value TBool
-  | Vlt    : value TInt -> value TInt -> value TBool
-  | Vge    : value TInt -> value TInt -> value TBool
-  | Vgt    : value TInt -> value TInt -> value TBool
-.
+  | VBool : bool -> value TBool
+  | VInt  : Z    -> value TInt.
+
+Definition const_to_value {ty} (c: const ty): value ty:=
+  match c with
+  | CBool b => VBool b
+  | CInt z => VInt z
+  end.
 
 Lemma value_inv {ty} (x: value ty) :
-  {c : const ty | x = VConst c} +
-  {eb : value TBool & {et : value ty & {ef : value ty | x = VIfte eb et ef}}} +
-  {e: value TInt | exists (eqt : TInt = ty), x = eq_rect _ value (Vnot e) _ eqt} +
-  {e: value TInt | exists (eqt : TInt = ty), x = eq_rect _ value (Vneg e) _ eqt} +
-  {e1: value TBool & {e2 : value TBool | exists (eqt : TBool = ty), x = eq_rect _ value (Vand e1 e2) _ eqt}} +
-  {e1: value TBool & {e2 : value TBool | exists (eqt : TBool = ty), x = eq_rect _ value (Vor e1 e2) _ eqt}} +
-  {e1: value TBool & {e2 : value TBool | exists (eqt : TBool = ty), x = eq_rect _ value (Vxor e1 e2) _ eqt}} +
-  {e1: value TInt & {e2 : value TInt | exists (eqt : TInt = ty), x = eq_rect _ value (Vplus e1 e2) _ eqt}} +
-  {e1: value TInt & {e2 : value TInt | exists (eqt : TInt = ty), x = eq_rect _ value (Vminus e1 e2) _ eqt}} +
-  {e1: value TInt & {e2 : value TInt | exists (eqt : TInt = ty), x = eq_rect _ value (Vmult e1 e2) _ eqt}} +
-  {e1: value TInt & {e2 : value TInt | exists (eqt : TInt = ty), x = eq_rect _ value (Vdiv e1 e2) _ eqt}} +
-  {e1: value TInt & {e2 : value TInt | exists (eqt : TBool = ty), x = eq_rect _ value (Veq e1 e2) _ eqt}} +
-  {e1: value TInt & {e2 : value TInt | exists (eqt : TBool = ty), x = eq_rect _ value (Vneq e1 e2) _ eqt}} +
-  {e1: value TInt & {e2 : value TInt | exists (eqt : TBool = ty), x = eq_rect _ value (Vle e1 e2) _ eqt}} +
-  {e1: value TInt & {e2 : value TInt | exists (eqt : TBool = ty), x = eq_rect _ value (Vlt e1 e2) _ eqt}} +
-  {e1: value TInt & {e2 : value TInt | exists (eqt : TBool = ty), x = eq_rect _ value (Vge e1 e2) _ eqt}} +
-  {e1: value TInt & {e2 : value TInt | exists (eqt : TBool = ty), x = eq_rect _ value (Vgt e1 e2) _ eqt}}.
+  {b : bool | exists (eqt : TBool = ty), x = eq_rect _ value (VBool b) _ eqt} +
+  {z : Z | exists (eqt : TInt = ty), x = eq_rect _ value (VInt z) _ eqt}.
 Proof using.
   destruct x.
-  1-16: left.
-  1-15: left.
-  1-14: left.
-  1-13: left.
-  1-12: left.
-  1-11: left.
-  1-10: left.
-  1-9: left.
-  1-8: left.
-  1-7: left.
-  1-6: left.
-  1-5: left.
-  1-4: left.
-  1-3: left.
-  1-2: left.
-  1-1: left.
-  2-17: right.
-  all: repeat (eexists; try exists eq_refl).
+  1: left.
+  2: right.
+  1: exists b.
+  2: exists z.
+  all: exists eq_refl.
+  all: reflexivity.
 Defined.
 
 Lemma value_dec {ty} (v1 v2: value ty) : {v1 = v2} + {v1 <> v2}.
 Proof.
-  revert v2.
-  induction v1 as [ty1 c1 | ty1 vb1 IHeb1 vt1 IHvt1 vf1 IHvf1 | v1 IH | v1 IH | v11 IH1 v12 IH2 | v11 IH1 v12 IH2 | v11 IH1 v12 IH2 | v11 IH1 v12 IH2 | v11 IH1 v12 IH2 | v11 IH1 v12 IH2 | v11 IH1 v12 IH2 | v11 IH1 v12 IH2 | v11 IH1 v12 IH2 | v11 IH1 v12 IH2 | v11 IH1 v12 IH2 | v11 IH1 v12 IH2 | v11 IH1 v12 IH2].
-  all: intro v2.
-  1, 2: destruct (value_inv v2) as [[[[[[[[[[[[[[[[
-    (c2 & ->) | (vb2 & vt2 & vf2 & ->)] |
-    (v2' & eqt2)] |
-    (v2' & eqt2)] |
-    (v21 & v22 & eqt2)] |
-    (v21 & v22 & eqt2)] |
-    (v21 & v22 & eqt2)] |
-    (v21 & v22 & eqt2)] |
-    (v21 & v22 & eqt2)] |
-    (v21 & v22 & eqt2)] |
-    (v21 & v22 & eqt2)] |
-    (v21 & v22 & eqt2)] |
-    (v21 & v22 & eqt2)] |
-    (v21 & v22 & eqt2)] |
-    (v21 & v22 & eqt2)] |
-    (v21 & v22 & eqt2)] |
-    (v21 & v22 & eqt2)]; try (right; (try destruct eqt2); subst; simpl; discriminate).
-  1: destruct (const_dec c1 c2); [left; subst; reflexivity | right; intros [=f]; apply sig2T_eq_type in f; contradiction].
-  1: destruct (IHeb1 vb2).
-  2: right; intros [=f]; contradiction.
-  1: destruct (IHvt1 vt2).
-  2: right; intros [=_ f]; apply sig2T_eq_type in f; contradiction.
-  1: destruct (IHvf1 vf2).
-  2: right; intros [=_ _ f]; apply sig2T_eq_type in f; contradiction.
-  1: subst; left; reflexivity.
-  1, 2: destruct (value_inv v2) as [[[[[[[[[[[[[[[[
-    (c2 & ->) | (vb2 & vt2 & vf2 & ->)] |
-    (v2' & eqt2)] |
-    (v2' & eqt2)] |
-    (v21 & v22 & eqt2)] |
-    (v21 & v22 & eqt2)] |
-    (v21 & v22 & eqt2)] |
-    (v21 & v22 & eqt2)] |
-    (v21 & v22 & eqt2)] |
-    (v21 & v22 & eqt2)] |
-    (v21 & v22 & eqt2)] |
-    (v21 & v22 & eqt2)] |
-    (v21 & v22 & eqt2)] |
-    (v21 & v22 & eqt2)] |
-    (v21 & v22 & eqt2)] |
-    (v21 & v22 & eqt2)] |
-    (v21 & v22 & eqt2)]; try (right; (try destruct eqt2); subst; simpl; discriminate); try (right; destruct eqt2 as [type_eq eqt2]; revert eqt2; refine (match type_eq with eq_refl => fun f => _ end); subst; discriminate).
-    1, 2: destruct (IH v2') as [eq|neq]; [left | right].
-    1-4: destruct eqt2 as [type_eq ->].
-    1, 3: exact (match type_eq with eq_refl => f_equal _ eq end).
-    1, 2: refine (match type_eq with eq_refl => fun f => _ end); cbn in f.
-    1, 2: injection f as f; exact (neq f).
-  all: destruct (value_inv v2) as [[[[[[[[[[[[[[[[
-    (c2 & ->) | (vb2 & vt2 & vf2 & ->)] |
-    (v2' & eqt2)] |
-    (v2' & eqt2)] |
-    (v21 & v22 & eqt2)] |
-    (v21 & v22 & eqt2)] |
-    (v21 & v22 & eqt2)] |
-    (v21 & v22 & eqt2)] |
-    (v21 & v22 & eqt2)] |
-    (v21 & v22 & eqt2)] |
-    (v21 & v22 & eqt2)] |
-    (v21 & v22 & eqt2)] |
-    (v21 & v22 & eqt2)] |
-    (v21 & v22 & eqt2)] |
-    (v21 & v22 & eqt2)] |
-    (v21 & v22 & eqt2)] |
-    (v21 & v22 & eqt2)]; try (right; (try destruct eqt2); subst; simpl; discriminate); try (right; destruct eqt2 as [type_eq eqt2]; revert eqt2; refine (match type_eq with eq_refl => fun f => _ end); subst; discriminate).
-    all: destruct (IH1 v21) as [eq1|neq1]; [| right].
-    all: try (destruct (IH2 v22) as [eq2|neq2]; [left| right]).
-    all: subst.
-    all: destruct eqt2 as [type_eq ->].
-    all: try exact (match type_eq with eq_refl => eq_refl end).
-    all: refine (match type_eq with eq_refl => fun f => _ end); cbn in f.
-    all: injection f as f.
-    all: contradiction.
+  destruct v1 as [b1 | z1].
+  all: destruct (value_inv v2) as [[b2 eqt2] | [z2 eqt2]].
+  2, 3: right; destruct eqt2; discriminate.
+  1: destruct (Bool.bool_dec b1 b2) as [eq | neq].
+  3: destruct (Z_noteq_dec z1 z2) as [neq | eq].
+  2, 3: right.
+  1, 4: left.
+  all: destruct eqt2 as [ ? [=->]]; subst.
+  all: rewrite (Eqdep_dec.UIP_dec type_dec x eq_refl).
+  all: cbn.
+  all: try reflexivity.
+  all: intro f; injection f.
+  all: intro; contradiction.
+Defined.
+
+Definition history := Dict.t {ty & Stream.t (value ty)}.
+Definition in_history (h : history) '((v, ty) : nat * type) := match Dict.find v h with
+  | Some (existT _ ty' _) => ty' = ty
+  | None => False
+end.
+Definition in_history' (h : history) '((v, ty) : nat * type) := exists s, Dict.find v h = Some (existT _ ty s).
+
+Lemma in_history_iff : forall h v, in_history h v <-> in_history' h v.
+Proof using.
+  intros h [ v ty ].
+  unfold in_history, in_history'.
+  destruct (Dict.find v h) as [ [ ty' e ] | ]; split.
+  - intros H.
+    subst.
+    exists e.
+    reflexivity.
+  - intros [ e' He ].
+    injection He as He.
+    exact (EqdepFacts.eq_sigT_fst H).
+  - intros [].
+  - intros [ e He ].
+    discriminate He.
 Qed.
+
+Definition extract_stream (ty : type) (t: nat) {ty'} (s : Stream.t (value ty')) : option (value ty) := match type_dec ty' ty with
+  | left e => Some (eq_rect ty' value (Stream.nth t s) ty e)
+  | right _ => None
+end.
+
+Lemma extract_stream_eqty : forall {ty} (s : Stream.t (value ty)) n, extract_stream ty n s = Some (Stream.nth n s).
+Proof using.
+  intros ty s n.
+  unfold extract_stream.
+  rewrite type_dec_same.
+  reflexivity.
+Qed.
+
+
+(* Operators *)
+Definition vnot (v: value TInt) : value TInt :=
+  match v with
+  | VInt z => VInt (1%Z - z)
+  end.
+
+Definition vneg (v: value TInt) : value TInt :=
+  match v with
+  | VInt z => VInt (-z)
+  end.
+
+Definition vand (v1 v2: value TBool) : value TBool :=
+  match v1, v2 with
+  | VBool b1, VBool b2 => VBool (b1 && b2)
+  end.
+
+Definition vor (v1 v2: value TBool) : value TBool :=
+  match v1, v2 with
+  | VBool b1, VBool b2 => VBool (b1 || b2)
+  end.
+
+Definition vxor (v1 v2: value TBool) : value TBool :=
+  match v1, v2 with
+  | VBool b1, VBool b2 => VBool (xorb b1 b2)
+  end.
+
+Definition vplus (v1 v2: value TInt) : value TInt :=
+  match v1, v2 with
+  | VInt z1, VInt z2 => VInt (z1 + z2)
+  end.
+
+Definition vminus (v1 v2: value TInt) : value TInt :=
+  match v1, v2 with
+  | VInt z1, VInt z2 => VInt (z1 - z2)
+  end.
+
+Definition vmult (v1 v2: value TInt) : value TInt :=
+  match v1, v2 with
+  | VInt z1, VInt z2 => VInt (z1 * z2)
+  end.
+
+Definition vdiv (v1 v2: value TInt) : value TInt :=
+  match v1, v2 with
+  | VInt z1, VInt z2 => VInt (z1 / z2)
+  end.
+
+Definition veq (v1 v2: value TInt) : value TBool :=
+  match v1, v2 with
+  | VInt z1, VInt z2 => VBool (Z.eqb z1 z2)
+  end.
+
+Definition vneq (v1 v2: value TInt) : value TBool :=
+  match v1, v2 with
+  | VInt z1, VInt z2 => VBool (negb (Z.eqb z1 z2))
+  end.
+
+Definition vle (v1 v2: value TInt) : value TBool :=
+  match v1, v2 with
+  | VInt z1, VInt z2 => VBool (Z.leb z1 z2)
+  end.
+
+Definition vlt (v1 v2: value TInt) : value TBool :=
+  match v1, v2 with
+  | VInt z1, VInt z2 => VBool (Z.ltb z1 z2)
+  end.
+
+Definition vge (v1 v2: value TInt) : value TBool :=
+  match v1, v2 with
+  | VInt z1, VInt z2 => VBool (Z.geb z1 z2)
+  end.
+
+Definition vgt (v1 v2: value TInt) : value TBool :=
+  match v1, v2 with
+  | VInt z1, VInt z2 => VBool (Z.gtb z1 z2)
+  end.
+
+Definition vifte {ty} (vb: value TBool) (vt vf: value ty) : value ty :=
+  match vb with
+  | VBool b => match b with
+    | true => vt
+    | false => vf
+    end
+  end.
